specIR/SIRhoareproof.v
@@ -1,0 +1,597 @@
+From Coq Require Import
+     Arith.PeanoNat
+     Lists.List
+     Strings.String
+     Morphisms
+     Setoid
+     RelationClasses.
+
+Require Import MapsC.
+Require Import ValuesC.
+Require Import MemoryC.
+Require Import CoqlibC.
+Require Import ASTC.
+Require Import EventsC.
+Require Import GlobalenvsC.
+Require Import IntegersC.
+Require Import Mod ModSem Any Skeleton.
+Require Import SimMem SimSymb Sound.
+Require SimMemId SimSymbId SoundTop.
+Require Import SimMod SimModSem.
+Require Import SIRCommon2 SIRmini.
+
+Require Import Program.
+Require Import Simulation.
+
+Set Implicit Arguments.
+
+
+
+Local Obligation Tactic := ii; ss; eauto.
+
+(*** TODO: move to SIRCommon ***)
+Lemma unfold_interp_mrec :
+forall (D E : Type -> Type) (ctx : forall T : Type, D T -> itree (D +' E) T) 
+  (R : Type) (t : itree (D +' E) R), interp_mrec ctx t = _interp_mrec ctx (observe t).
+Proof.
+  i. f. eapply unfold_interp_mrec; et.
+Qed.
+
+Lemma bind_ret_l : forall (E : Type -> Type) (R S : Type) (r : R) (k : R -> itree E S),
+    ` x : _ <- Ret r;; k x = k r.
+Proof.
+  i. f. eapply bind_ret_l.
+Qed.
+
+Lemma bind_ret_r : forall (E : Type -> Type) (R : Type) (s : itree E R), ` x : R <- s;; Ret x = s.
+Proof.
+  i. f. eapply bind_ret_r.
+Qed.
+
+Lemma bind_tau : forall (E : Type -> Type) (R U : Type) (t : itree E U) (k : U -> itree E R),
+  ` x : _ <- Tau t;; k x = Tau (` x : _ <- t;; k x).
+Proof.
+  i. f. eapply bind_tau.
+Qed.
+
+Lemma bind_vis: forall (E : Type -> Type) (R U V : Type) (e : E V) (ek : V -> itree E U) (k : U -> itree E R),
+  ` x : _ <- Vis e ek;; k x = Vis e (fun x : V => ` x : _ <- ek x;; k x).
+Proof.
+  i. f. eapply bind_vis.
+Qed.
+
+
+
+
+
+Section OWNEDHEAP.
+
+Variable mi: string.
+Variable owned_heap: Type.
+Variable X: Type.
+Variable precond: forall (oh0: owned_heap) (m0: mem) (vs: list val), option X.
+Variable postcond: forall (oh0: owned_heap) (m0: mem) (vs: list val) (x: X), (owned_heap * (mem * val)) -> Prop.
+
+
+
+
+(*** sim syntax ***)
+Section SYNTAX.
+
+(*** sim itree ***)
+Let itr := itree (E owned_heap) (owned_heap * (mem * val)).
+
+Inductive _sim_itr (sim_itr: itr -> itr -> Prop): itr -> itr -> Prop :=
+| sim_ret
+    oh m v
+  :
+    _sim_itr sim_itr (Ret (oh, (m, v))) (Ret (oh, (m, v)))
+| sim_tau
+    i_src
+    i_tgt
+    (SIM: sim_itr i_src i_tgt)
+  :
+    _sim_itr sim_itr (Tau i_src) (Tau i_tgt)
+| sim_icall
+    fname oh m vs
+    k_src
+    k_tgt
+    (SIM: (eq ==> sim_itr)%signature k_src k_tgt)
+  :
+    _sim_itr sim_itr
+             (Vis (subevent _ (ICall fname oh m vs)) k_src)
+             (Vis (subevent _ (ICall fname oh m vs)) k_tgt)
+| sim_ecall
+    sg oh m vs fptr
+    k_src
+    k_tgt
+    (SIM: (eq ==> sim_itr)%signature k_src k_tgt)
+  :
+    _sim_itr sim_itr
+             (Vis (subevent _ (ECall sg fptr oh m vs)) k_src)
+             (Vis (subevent _ (ECall sg fptr oh m vs)) k_tgt)
+| sim_nb
+    i_src k_tgt
+  :
+    _sim_itr sim_itr i_src (Vis (subevent _ (ENB)) k_tgt)
+| sim_ub
+    k_src i_tgt
+  :
+    _sim_itr sim_itr (Vis (subevent _ (EUB)) k_src) i_tgt
+| sim_choose
+    X
+    k_src k_tgt
+    (SIM: (eq ==> sim_itr)%signature k_src k_tgt)
+  :
+    _sim_itr sim_itr
+             (Vis (subevent _ (EChoose X)) k_src)
+             (Vis (subevent _ (EChoose X)) k_tgt)
+.
+
+Definition sim_itr: itr -> itr -> Prop := paco2 _sim_itr bot2.
+
+Lemma sim_itr_mon: monotone2 _sim_itr.
+Proof.
+  ii. inv IN; try econs; et; rr; et.
+Unshelve.
+Qed.
+Hint Unfold sim_itr.
+Hint Resolve sim_itr_mon: paco.
+
+
+
+Let fn_src := function owned_heap_src.
+Let fn_tgt := function owned_heap_tgt.
+
+(*** TODO: curry "function", and we can state "SALL --> sim_itr" ***)
+(*** TODO: give better name than SALL ***)
+Definition sim_fn (k_src: fn_src) (k_tgt: fn_tgt): Prop := forall
+    m vs
+    oh_src oh_tgt
+    (O: SO oh_src oh_tgt)
+  ,
+    <<SIM: sim_itr (k_src oh_src m vs) (k_tgt oh_tgt m vs)>>
+.
+
+
+
+
+
+(*** sim prog ***)
+Definition sim_prog: program owned_heap_src -> program owned_heap_tgt -> Prop :=
+  eq !-> option_rel sim_fn
+.
+
+
+
+
+(*** useful lemma for below proof ***)
+(*** copied from "eqit_bind_clo" in itree repo - Eq.v ***)
+Inductive bindC (r: itr_src -> itr_tgt -> Prop) : itr_src -> itr_tgt -> Prop :=
+| bindC_intro
+    i_src i_tgt
+    (SIM: sim_itr i_src i_tgt)
+    k_src k_tgt
+    (SIMK: HProper (SALL !-> r) k_src k_tgt)
+    (* (SIMK: forall *)
+    (*     oh_src oh_tgt m vs *)
+    (*     (O: SO oh_src oh_tgt) *)
+    (*   , *)
+    (*     <<SIM: r (k_src (oh_src, (m, vs))) (k_tgt (oh_tgt, (m, vs)))>>) *)
+  :
+    bindC r (ITree.bind i_src k_src) (ITree.bind i_tgt k_tgt)
+.
+
+Hint Constructors bindC: core.
+
+Lemma bindC_spec
+      simC
+  :
+    bindC <3= gupaco2 (_sim_itr) (simC)
+.
+Proof.
+  gcofix CIH. intros. destruct PR.
+  punfold SIM. inv SIM.
+  - rewrite ! bind_ret_l. gbase. eapply SIMK; et. rr; et.
+  - rewrite ! bind_tau. gstep. econs; eauto. pclearbot.
+    (* gfinal. left. eapply CIH. econstructor; eauto. *)
+    debug eauto with paco.
+  - rewrite ! bind_vis. gstep. econs; eauto. u. ii. repeat spc SIM0. pclearbot.
+    (* gfinal. left. eapply CIH. econs. { et. } uh. ii. eapply SIMK. et. *)
+    eauto with paco.
+  - rewrite ! bind_vis. gstep. econs; eauto. u. ii. repeat spc SIM0. pclearbot.
+    eauto with paco.
+  - rewrite ! bind_vis. gstep. econs; eauto.
+  - rewrite ! bind_vis. gstep. econs; eauto.
+  - rewrite ! bind_vis. rewrite ! bind_tau.
+    gstep. econs; eauto. des. pclearbot. eauto with paco.
+  - rewrite ! bind_vis. rewrite ! bind_tau.
+    gstep. econs; eauto. ii. pclearbot. eauto with paco.
+Qed.
+
+Global Instance sim_itr_bind :
+  HProper ((SALL !-> sim_itr) !-> sim_itr !-> sim_itr) ITree.bind' ITree.bind'
+.
+Proof.
+  red. ginit.
+  { intros. eapply cpn2_wcompat; eauto with paco. }
+  guclo bindC_spec. ii. econs; et.
+  u. ii.
+  exploit H0; et.
+  intro T. eauto with paco.
+Qed.
+
+End SYNTAX.
+Hint Unfold sim_itr.
+Hint Resolve sim_itr_mon: paco.
+
+
+
+
+
+
+
+
+
+(*** sim semantics ***)
+Section SEMANTICS.
+
+(*** sim states ***)
+Let st_src := (SIRmini.state owned_heap_src).
+Let st_tgt := (SIRmini.state owned_heap_tgt).
+
+Inductive _sim_st (sim_st: st_src -> st_tgt -> Prop): st_src -> st_tgt -> Prop :=
+| sim_st_ret
+    oh_src oh_tgt m v
+    (O: SO oh_src oh_tgt)
+  :
+    _sim_st sim_st (Ret (oh_src, (m, v))) (Ret (oh_tgt, (m, v)))
+| sim_st_tau
+    i_src
+    i_tgt
+    (SIM: sim_st i_src i_tgt)
+  :
+    _sim_st sim_st (Tau i_src) (Tau i_tgt)
+| sim_st_ecall
+    sg m vs fptr
+    oh_src k_src
+    oh_tgt k_tgt
+    (O: SO oh_src oh_tgt)
+    (SIM: HProper (SALL !-> sim_st) k_src k_tgt)
+  :
+    _sim_st sim_st
+             (Vis (subevent _ (ECall sg fptr oh_src m vs)) k_src)
+             (Vis (subevent _ (ECall sg fptr oh_tgt m vs)) k_tgt)
+| sim_st_nb
+    i_src k_tgt
+  :
+    _sim_st sim_st i_src (Vis (subevent _ (ENB)) k_tgt)
+| sim_st_ub
+    k_src i_tgt
+  :
+    _sim_st sim_st (Vis (subevent _ (EUB)) k_src) i_tgt
+| sim_st_choose_src
+    X_src
+    k_src i_tgt
+    (SIM: exists x_src, sim_st (k_src x_src) i_tgt)
+  :
+    _sim_st sim_st
+            (Vis (subevent _ (EChoose X_src)) k_src)
+            (Tau i_tgt)
+| sim_st_choose_tgt
+    X_tgt
+    k_tgt i_src
+    (INHAB: inhabited X_tgt)
+    (SIM: forall x_tgt, sim_st i_src (k_tgt x_tgt))
+  :
+    _sim_st sim_st
+            (Tau i_src)
+            (Vis (subevent _ (EChoose X_tgt)) k_tgt)
+.
+
+Definition sim_st: st_src -> st_tgt -> Prop := paco2 _sim_st bot2.
+
+Lemma sim_st_mon: monotone2 _sim_st.
+Proof.
+  ii. inv IN; try econs; et.
+  des. esplits; et.
+Unshelve.
+Qed.
+Hint Unfold sim_st.
+Hint Resolve sim_st_mon: paco.
+
+End SEMANTICS.
+Hint Unfold sim_st.
+Hint Resolve sim_st_mon: paco.
+
+
+
+
+
+
+
+
+Section SIM.
+
+  Variable p_src: program owned_heap_src.
+  Variable p_tgt: program owned_heap_tgt.
+  Hypothesis (SIMP: sim_prog p_src p_tgt).
+
+  Lemma sim_prog_sim_st
+        i_src i_tgt
+        (SIM: sim_itr i_src i_tgt)
+    :
+      sim_st (interp_mrec (interp_function p_src) i_src)
+             (interp_mrec (interp_function p_tgt) i_tgt)
+  .
+  Proof.
+    revert_until SIMP.
+    ginit.
+    { intros. eapply cpn2_wcompat; et. eauto with paco. }
+    gcofix CIH.
+    i. rewrite ! unfold_interp_mrec.
+    punfold SIM. inv SIM; cbn.
+    - gstep. econs; et.
+    - pclearbot. gstep. econs; et. gbase. et.
+    - pclearbot. gstep. econs; et. gbase.
+      eapply CIH. eapply sim_itr_bind.
+      { u. ii. repeat spc SIM0. pclearbot. eauto. }
+      exploit (@SIMP fname); et. intro T.
+      inv T.
+      { pfold. econs; et. }
+      exploit H1; et.
+    - gstep. econs; et. u in *. gstep. econs; et. repeat spc SIM0. des; ss. gbase. eapply CIH.
+      eauto with paco.
+    - gstep. econs; et.
+    - gstep. econs; et.
+    - gstep. des. pclearbot. econs; et. esplits; et. gstep.
+      rewrite (unfold_interp_mrec _ (Tau i_tgt0)). cbn. econs; et. eauto with paco.
+    - gstep. pclearbot. econs; et. ii. repeat spc SIM0. gstep.
+      rewrite (unfold_interp_mrec _ (Tau i_src0)). cbn. econs; et. eauto with paco.
+  Qed.
+
+  (*** The result that we wanted -- allows reasoning each function "locally" and then compose ***)
+  Theorem adequacy_local_local:
+    forall
+      (fname: ident) m vs oh_src oh_tgt
+      (O: SO oh_src oh_tgt)
+    ,
+      (<<SIM: sim_st (interp_program0 p_src (ICall fname oh_src m vs))
+                     (interp_program0 p_tgt (ICall fname oh_tgt m vs))
+                     >>)
+  .
+  Proof.
+    {
+      ii.
+      eapply sim_prog_sim_st; ss.
+      hexploit (@SIMP fname); et. intro T. inv T; ss.
+      { pfold. econs; et. }
+      repeat (spc H1). des. ss.
+    }
+  Qed.
+
+  (*** lifting above proof into small-step semantics ***)
+  Section SMO.
+
+    Record t: Type :=
+      mk {
+          sm :> SimMem.t;
+          oh_src: Any;
+          oh_tgt: Any;
+        }
+    .
+
+    Inductive wf (smo: t): Prop :=
+    | wf_intro
+        (o_src: owned_heap_src) (o_tgt: owned_heap_tgt)
+        (MWF: SimMem.wf smo)
+        (OHSRC: smo.(oh_src) = upcast o_src)
+        (OHTGT: smo.(oh_tgt) = upcast o_tgt)
+        (O: SO o_src o_tgt)
+    .
+
+    Local Obligation Tactic := try (by ii; des; ss).
+
+    Program Instance SimMemOh: (SimMemOh.class) :=
+      {|
+      SimMemOh.t := t;
+      SimMemOh.sm := sm;
+      SimMemOh.oh_src := oh_src;
+      SimMemOh.oh_tgt := oh_tgt;
+      SimMemOh.wf := wf;
+      SimMemOh.le := SimMem.le;
+      SimMemOh.lepriv := SimMem.lepriv;
+      SimMemOh.midx := Some mi;
+      SimMemOh.set_sm := fun smo sm => mk sm smo.(oh_src) smo.(oh_tgt);
+      |}
+    .
+    Next Obligation.
+      ii. eapply PR.
+    Qed.
+    Next Obligation.
+      ii. inv WF.
+      econs; ss; et.
+    Qed.
+    Next Obligation.
+      ss. ii. destruct smo0; ss.
+    Qed.
+
+  End SMO.
+
+  Variable ioh_src: SkEnv.t -> owned_heap_src.
+  Variable ioh_tgt: SkEnv.t -> owned_heap_tgt.
+  Hypothesis (SIMO: forall skenv, SO (ioh_src skenv) (ioh_tgt skenv)).
+  Variable sk: Sk.t.
+  Let md_src: Mod.t := (SIRmini.module sk p_src mi ioh_src).
+  Let md_tgt: Mod.t := (SIRmini.module sk p_tgt mi ioh_tgt).
+
+
+
+  (*** Lifting to SimModSem ***)
+  Section SIMMODSEM.
+
+    Variable skenv_link: SkEnv.t.
+    Variable sm_link: SimMem.t.
+    Let ms_src: ModSem.t := (Mod.modsem md_src skenv_link).
+    Let ms_tgt: ModSem.t := (Mod.modsem md_tgt skenv_link).
+    Hypothesis (INCL: SkEnv.includes skenv_link (Mod.sk md_src)).
+    Hypothesis (WF: SkEnv.wf skenv_link).
+
+    Local Existing Instance SimMemOh.
+    Local Arguments ModSemPair.mk [SM] [SS] _ _ _ _ [SMO].
+
+    Definition msp: ModSemPair.t := ModSemPair.mk (md_src skenv_link) (md_tgt skenv_link)
+                                                  (SimSymbId.mk md_src md_tgt) sm_link.
+
+    Inductive match_states (idx: nat): SIRmini.state owned_heap_src ->
+                                       SIRmini.state owned_heap_tgt -> SimMemOh.t -> Prop :=
+    | match_states_intro
+        st_src st_tgt smo0
+        (SIM: sim_st st_src st_tgt)
+        (MWF: SimMemOh.wf smo0)
+      :
+        match_states idx st_src st_tgt smo0
+    .
+
+    Lemma match_states_lxsim
+          idx st_src_src st_tgt_src smo_src
+          (MATCH: match_states idx st_src_src st_tgt_src smo_src)
+      :
+        <<XSIM: lxsim (md_src skenv_link) (md_tgt skenv_link)
+                      (fun _ => () -> exists (_ : ()) (_ : mem), True)
+                      (Ord.lift_idx lt_wf idx) st_src_src st_tgt_src smo_src>>
+    .
+    Proof.
+      revert_until idx. revert idx.
+      ginit.
+      { intros. eapply cpn4_wcompat; eauto with paco. }
+      gcofix CIH. i. gstep.
+      ii. clear SUSTAR.
+
+      inv MATCH. ss.
+      punfold SIM. inv SIM.
+      - assert(U:=MWF).
+        inv MWF. inv MWF0. destruct smo_src; ss. destruct sm0; ss. clarify.
+        econstructor 4 with (smo_ret := mk (SimMemId.mk m m)
+                                           (upcast oh_src0) (upcast oh_tgt0)); ss; eauto.
+        + econs; ss; et.
+        + econs; ss; et.
+        + econs; ss; et.
+        + rr. ss. esplits; ss; et.
+          { econs; ss; et. }
+      - (* TAU *)
+        econs 1; et.
+        econs 1; et; swap 2 3.
+        { split; intro T; rr in T; des; ss; inv T; ss. }
+        { eapply modsem_receptive; et. }
+        ii; ss. inv STEPSRC; ss. clarify. esplits; ss; et.
+        { left. eapply plus_one. rr. esplits; et.
+          { eapply modsem_determinate; ss; et. }
+          econs; et.
+        }
+        pclearbot. gbase. eapply CIH. econs; et.
+      - (* ECALL *)
+        econs 3; et.
+        { admit "TODO: fix -- ~step, ~ret should suffice". }
+        ii; ss. inv ATSRC. csc.
+        eexists _, _, (mk (SimMemId.mk m0 m0) (upcast oh_src1) (upcast oh_tgt0)); ss.
+        esplits; ss; et.
+        { rr. ss. esplits; ss; et. econs; ss; et. }
+        { econs; ss; et. }
+        { econs; ss; et. }
+        ii. des. inv AFTERSRC; ss. inv GETK; ss. csc.
+        rename oh_src0 into oh_src1.
+        rename _oh0 into oh_src0.
+        rr in SIMRETV. des; ss. inv SIMRETV0; ss. clarify.
+        inv MWF0. ss. destruct smo_ret; ss. destruct sm0; ss. subst. clarify. clear_tac.
+        esplits; et.
+        { econs; ss; et. econs; ss; et. }
+        u in SIM0.
+        hexploit SIM0; et.
+        { instantiate (2:= (o_src, (_, _))). instantiate (1:= (o_tgt, (_, _))). ss. }
+        intro T. des; ss.
+        gbase. eapply CIH. econs; et.
+      - (* NB *)
+        econs 2; ss; et. ii.
+        econs 3; ss; et.
+        { ii; ss. inv STEPTGT; ss. }
+        { esplits; et. econsby ss. }
+      - (* UB *)
+        econs 2; ss; et. ii.
+        exploit SAFESRC; et.
+        { eapply star_refl. }
+        intro T; des; ss.
+        + rr in EVCALL. des; ss. inv EVCALL; ss.
+        + rr in EVRET. des; ss. inv EVRET; ss.
+        + inv EVSTEP; ss.
+      - (* CHOOSE SRC *)
+        des. pclearbot.
+        econs 2; ss; et. ii.
+        econs 1; ss; et; cycle 1.
+        { esplits; ss; et. econs; ss; et. }
+        { ii. inv STEPTGT; ss; clarify. esplits; et.
+          + left. eapply plus_one. econs 3; ss; et.
+          + gbase. eapply CIH. econs; et.
+        }
+      - (* CHOOSE TGT *)
+        des. pclearbot. inv INHAB.
+        econs 2; ss; et. ii.
+        econs 1; ss; et; cycle 1.
+        { esplits; ss; et. econs 3; ss; et. }
+        { ii. inv STEPTGT; ss; csc. esplits; et.
+          + left. eapply plus_one. econs; ss; et.
+          + gbase. eapply CIH. econs; et.
+        }
+    Unshelve.
+      all: ss.
+      all: try (econsby ss).
+    Qed.
+
+    Theorem sim_modsem: ModSemPair.sim msp.
+    Proof.
+      econstructor 1 with (sidx := unit) (sound_states := top4); eauto;
+        try apply SoundTop.sound_state_local_preservation; et; try (by ii; ss).
+      { ii. eapply Preservation.local_preservation_noguarantee_weak.
+        apply SoundTop.sound_state_local_preservation; et.
+      }
+      { ii. ss. eexists (mk _ _ _); ss. esplits; eauto. econs; ss; eauto. }
+      ii. ss. esplits; eauto.
+      - ii. des. inv INITTGT. inv SAFESRC. ss. des_ifs_safe.
+        esplits; eauto.
+        { econs; ss; et. }
+        eapply match_states_lxsim; eauto.
+        econs; ss; et.
+        eapply sim_prog_sim_st; et.
+        rr in SIMARGS. des. inv SIMARGS0; ss. clarify. inv MWF. ss. destruct sm_arg; ss.
+        destruct sm0; ss. subst. clarify. clear_tac.
+        assert(fid0 = fid).
+        { apply_all_once Genv.find_invert_symbol. clarify. }
+        clarify.
+        rr in SIMP. repeat spc SIMP. hexploit1 SIMP; et. inv SIMP; ss.
+        { pfold. econs; et. }
+        { eapply H1; et. }
+      - i; des. inv SAFESRC. ss. des_ifs.
+        rr in SIMARGS. des. inv SIMARGS0; ss. clarify. destruct sm_arg; ss. destruct sm0; ss. clarify.
+        esplits; et. econs; ss; et.
+    Unshelve.
+      all: ss.
+      all: try (econsby ss).
+    Qed.
+
+  End SIMMODSEM.
+
+  Theorem sim_mod: ModPair.sim (SimSymbId.mk_mp (SIRmini.module sk p_src mi ioh_src)
+                                                (SIRmini.module sk p_tgt mi ioh_tgt)).
+  Proof.
+    ii. econs; ss; eauto.
+    ii. rr in SIMSKENVLINK. clarify. esplits. eapply sim_modsem; et.
+  Qed.
+
+End SIM.
+
+End OWNEDHEAP.
+Hint Unfold sim_itr.
+Hint Resolve sim_itr_mon: paco.
+Hint Constructors bindC: core.
+Hint Unfold sim_st.
+Hint Resolve sim_st_mon: paco.
